implementing upd_even and upd_odd, assuming definitions from nik_fictional

pulse/ulib/experimental/Steel.Stepper.fst
@@ -18,6 +18,8 @@ type stepper =
   | OddWriteable : odd -> stepper
   | None : stepper
 
+let refine (s:stepper) = V? s \/ None? s
+
 let composable' (s0 s1:stepper) : prop =
     match s0, s1 with
     | _, None
@@ -88,8 +90,6 @@ let frame_compatible (x:erased stepper) (v y:stepper) =
             composable y frame /\
             v == compose y frame)
 
-let refine v = V? v \/ None? v
-
 
 assume
 val select_refine (r:ref stepper p)
@@ -101,6 +101,50 @@ val select_refine (r:ref stepper p)
              (pts_to r x)
              (fun v -> pts_to r (f v))
 
+
+(** Updating a ref cell for a user-defined PCM *)
+
+(** A frame-preserving update set on a PCM p, specified in two
+    parts:
+
+    1. To update a share of a PCM from [x] to [y]:
+        - Given a full value [v] compatible with [x] (i.e. exists f. op p x f = v)
+
+        + Produce a value [z] compatible with [y] (i.e.,
+          the final heap satisfies [pts_to r y])
+
+          - if v is a refined value then so is z,
+            and respects the preorder of frame_preserving updates on refined values
+*)
+let frame_preserving_upd_0 (x y:stepper) =
+    v:stepper{compatible p x v}
+  -> Tot (z:stepper{
+            compatible p y z /\
+             (refine v ==> refine z) /\
+             (refine v ==> frame_preserving p v z)})
+
+(** Further, the update respects PCM frames:
+
+    For any [frame] composable with the value [v] being updated,
+    [f] only updates the [v] part of [op p v frame] to [z], obtaining
+    [op p z frame]
+ *)
+let frame_preserving_upd (x y:stepper) =
+  f:frame_preserving_upd_0 x y {
+     forall (v:stepper{compatible p x v}).
+         let z = f v in
+         (forall (frame:stepper). {:pattern (FStar.PCM.composable p v frame)}
+              FStar.PCM.composable p v frame ==>
+              FStar.PCM.composable p z frame /\
+              (compatible p x (op p v frame) ==>
+              (op p z frame == f (op p v frame))))
+  }
+
+assume
+val upd_gen_action (r:ref stepper p)
+                   (x y:Ghost.erased stepper)
+                   (f:frame_preserving_upd x y)
+  : SteelT unit (pts_to r x) (fun _ -> pts_to r y)
 
 let f_even (n0:even) (v:stepper{compatible p (Even n0) v})
   : GTot (y:stepper{compatible p y v /\ frame_compatible (Even n0) v y})
@@ -156,13 +200,36 @@ let get_odd (r:ref stepper p) (n0:odd)
     change_slprop (pts_to r (f_odd n0 v)) (if n = n0 then pts_to r (Odd n0) else pts_to r (OddWriteable n0)) (fun _ -> ());
     n
 
-assume
-val upd_even (r:ref stepper p) (n:even) :
-  SteelT unit (pts_to r (EvenWriteable n)) (fun _ -> pts_to r (Even (n+2)))
+let upd_even_f (n:even) : frame_preserving_upd (EvenWriteable n)
+                                               (Even (n + 2))
+  = let f
+      : frame_preserving_upd_0 (EvenWriteable n) (Even (n + 2))
+      = function
+        | EvenWriteable n -> Even (n + 2)
+        | V n -> V (n + 1)
+    in
+    f
 
-assume
-val upd_odd (r:ref stepper p) (n:odd) :
-  SteelT unit (pts_to r (OddWriteable n)) (fun _ -> pts_to r (Odd (n+2)))
+let upd_odd_f (n:odd) : frame_preserving_upd (OddWriteable n) (Odd (n + 2))
+  = let f
+      : frame_preserving_upd_0 (OddWriteable n) (Odd (n + 2))
+      = function
+        | OddWriteable n -> Odd (n + 2)
+        | V n -> V (n + 1)
+    in
+    f
+
+let upd_even (r:ref stepper p) (n:even)
+  : SteelT unit (pts_to r (EvenWriteable n)) (fun _ -> pts_to r (Even (n+2)))
+  = upd_gen_action r (Ghost.hide (EvenWriteable n))
+                     (Ghost.hide (Even (n + 2)))
+                     (upd_even_f n)
+
+let upd_odd (r:ref stepper p) (n:odd)
+  : SteelT unit (pts_to r (OddWriteable n)) (fun _ -> pts_to r (Odd (n+2)))
+  = upd_gen_action r (Ghost.hide (OddWriteable n))
+                     (Ghost.hide (Odd (n + 2)))
+                     (upd_odd_f n)
 
 assume
 val alloc (x:stepper{compatible p x x})
